Very broken hamster

Validation/Dafny/Hamster.dfy
@@ -1,79 +1,79 @@
-trait PointT {
+class {:autocontracts} PointT {
   var x: int
   var y: int
 
-  method Clone() 
-    returns (p: PointT) 
-    ensures fresh(p)
+  function method Valid(): bool ensures Valid() reads {} { true }
+	constructor (xx: int, yy: int) { x := xx; y := yy;  }
 
-  function method Equal(p: PointT): 
-    bool reads this, p ensures this == p ==> this.Equal(p)
-}
-
-class Point extends PointT
-{
-
-  constructor (xx: int, yy: int) { x := xx; y := yy;  }
   function method Equal(p: PointT): bool 
-    reads this, p ensures this == p ==> this.Equal(p) 
+    reads this, p, this.Repr
   {
     this.x == p.x && this.y == p.y 
   }
-  method Clone() returns (p: PointT) ensures fresh(p) 
-  {
-      p := new Point(x, y);
-  }
 }
 
-method {:opaque} Assume(b: bool) decreases * ensures b 
-{
-  if !b 
-  {
-    print "Asssumption failed!";
-    while (true) decreases * { }
-  }
-}
 
-class Hamster {
+method  Check(b: bool) decreases * ensures b { if !b { print "Asssumption failed!"; while true decreases * { } } }
+function method {:verify false} Assume(b: bool): () ensures b { () }
+
+class {:autocontracts} Hamster {
   var pos: PointT
-  constructor (p: PointT) { this.pos := p; }
+  constructor (p: PointT) { this.pos := new PointT(p.x, p.y); }
 }
 
 type Path = array<PointT>
-class {:autocontracts} Cage
+class /*{:autocontracts}*/ Cage
 {
-  var path: Path
-  var h: Hamster
+	ghost var Repr: set<object?> // GENERATED
+	var path: Path
+	var h: Hamster
 
-  constructor (h: Hamster, path: Path) decreases *
-  {
-    this.h := new Hamster(h.pos);   
-    this.path := new PointT[path.Length](
-      (i : nat) reads path requires i < path.Length => path[i]
-    );
-    new;
-    Assume(this.Valid());
-  }
+	constructor (h: Hamster, path: Path) decreases *
+		//requires exists p : PointT | p in path[..] :: p.Equal(h.pos)
+		ensures fresh({this.h, this.path})
+		modifies this // GENERATED
+		ensures this.Valid() // GENERATED
+		ensures fresh(Repr - {this}) // GENERATED
+	{
+		this.h := new Hamster(h.pos);   
+		this.path := new PointT[path.Length](
+			(i : nat) reads path requires i < path.Length => path[i]
+		);
+		new;
+				
+		this.Repr := {this}; // GENERATED
+		if (this.path !in Repr) { Repr := Repr + {this.path}; } // GENERATED
+		if (this.h !in Repr) { Repr := Repr + {this.h}; } // GENERATED
 
-  function method Valid(): bool 
-    reads this, this.h, this.h.pos, this.path, this.path[..] 
-    reads this, Repr
-  {
-    exists p : PointT | p in this.path[..] :: p.Equal(this.h.pos)
-  }
+		Check(this.Valid()); // I need to add this here (after the above lines)
+		var _ := Assume(this.Valid());
+	}
 
-  method Move()
-    decreases *
-    modifies this, this.h, this.h.pos
-  { 
+	function method Valid(): bool 
+		reads this, this.h, this.h.pos, this.path, this.path[..] 
+		reads this, this.Repr // GENERATED
+	{
+		//forall p:  PointT | p in this.path[..] :: p.Valid() &&
+		exists p : PointT | p in this.path[..] :: p.Equal(this.h.pos)
+	}
+
+	method Move() modifies this.h, this.h.pos
+		decreases *
+		ensures this.h == old(this.h)
+		ensures this.h.pos in this.path[..]
+		requires this.Valid() // GENERATED
+		ensures this.Valid() // GENERATED
+		ensures fresh(this.Repr - old(this.Repr)) // GENERATED
+	{ 
 		var index := 1;
 		while index <= this.path.Length && !this.path[index - 1].Equal(this.h.pos) { 
-      index := index + 1;
-    }
+			index := index + 1;
+		}
 
-    //assert this.path.Length > 0;
+		//assert this.path.Length > 0;
 		this.h.pos := this.path[index % this.path.Length];
-    Assume(this.Valid());
+		Check(this.Valid());
+		var _ := Assume(this.Valid()); // This should be unnecessary...
 	}
 }
 
@@ -81,21 +81,21 @@ method Main()
   decreases *
 {
   print "hello, Dafny\n";
-  var p0 := new Point(0, 0);
-  var p1 := new Point(2, 2);
-  var p2 := new Point(0, 0);
+  var p0 := new PointT(0, 0);
+  var p1 := new PointT(2, 2);
+  var p2 := new PointT(0, 0);
   var pl := new PointT[3][p0, p1, p2];
 
-  var ph := new Point(0, 0);
+  var ph := new PointT(0, 0);
   var h := new Hamster(ph);
   var c := new Cage(h, pl);
 
-//  Assume(c.h.pos.x == 0 && c.h.pos.y == 0);
+//  Check(c.h.pos.x == 0 && c.h.pos.y == 0);
   c.Move();
- // Assume(c.h.pos.x == 2 && c.h.pos.y == 2);
+ // Check(c.h.pos.x == 2 && c.h.pos.y == 2);
   c.Move();
- // Assume(c.h.pos.x == 0 && c.h.pos.y == 0);
+ // Check(c.h.pos.x == 0 && c.h.pos.y == 0);
   c.Move();
-// Assume(c.h.pos.x == 2 && c.h.pos.y == 2);
+// Check(c.h.pos.x == 2 && c.h.pos.y == 2);
   //PlayWith(c);
 }
